coq/Translation/NNRCtoNNRCimp.v
@@ -115,6 +115,15 @@ Section NNRCtoNNRCimp.
           rewrite eqq; trivial.
     Qed.
 
+    Corollary nnrc_expr_to_nnrc_imp_expr_some_correct'
+              (e:nnrc) (ei:nnrc_imp_expr) :
+      nnrc_expr_to_nnrc_imp_expr e = Some ei ->
+      forall h σc σ,
+        @nnrc_core_eval _ h σc σ (nnrc_to_nnrc_base e) = nnrc_imp_expr_eval h σc (pd_bindings_lift σ) ei.
+    Proof.
+      apply nnrc_expr_to_nnrc_imp_expr_some_correct.
+    Qed.
+
     Inductive terminator :=
     | Term_assign : var -> terminator
     | Term_push : var -> terminator
@@ -130,8 +139,8 @@ Section NNRCtoNNRCimp.
       option nnrc_imp_stmt
       := match stmt with
          | NNRCLet v s1 s2 =>
-           match nnrc_stmt_to_nnrc_imp_stmt_aux (v::fvs) (Term_assign v) s1,
-                 nnrc_stmt_to_nnrc_imp_stmt_aux (v::fvs) terminator s2
+           match nnrc_stmt_to_nnrc_imp_stmt_aux fvs (Term_assign v) s1,
+                 nnrc_stmt_to_nnrc_imp_stmt_aux fvs terminator s2
            with
            | Some s1', Some s2' =>
              Some (NNRCimpLetMut v s1' s2')
@@ -140,39 +149,31 @@ Section NNRCtoNNRCimp.
          | NNRCFor v e s =>
            let tmp := fresh_var "tmp" fvs in
            match nnrc_expr_to_nnrc_imp_expr e,
-                 nnrc_stmt_to_nnrc_imp_stmt_aux (tmp::v::fvs) (Term_push tmp) s
+                 nnrc_stmt_to_nnrc_imp_stmt_aux (tmp::fvs) (Term_push tmp) s
            with
            | Some e', Some s' =>
-             Some (NNRCimpLetMut
+             Some (NNRCimpLetMutColl
                      tmp
                      (NNRCimpFor v e' s')
                      (terminate terminator (NNRCimpVar tmp)))
            | _, _ => None
            end
          | NNRCIf e s1 s2 =>
-           let tmp := fresh_var "tmp" fvs in
            match nnrc_expr_to_nnrc_imp_expr e,
-                 nnrc_stmt_to_nnrc_imp_stmt_aux (tmp::fvs) (Term_assign tmp) s1,
-                 nnrc_stmt_to_nnrc_imp_stmt_aux (tmp::fvs) (Term_assign tmp) s2
+                 nnrc_stmt_to_nnrc_imp_stmt_aux fvs terminator s1,
+                 nnrc_stmt_to_nnrc_imp_stmt_aux fvs terminator s2
            with
            | Some e', Some s1', Some s2' =>
-             Some (NNRCimpLetMut
-                     tmp 
-                        (NNRCimpIf e' s1' s2')
-                        (terminate terminator (NNRCimpVar tmp)))
+             Some (NNRCimpIf e' s1' s2')
            | _, _, _ => None
            end
          | NNRCEither e x1 s1 x2 s2 =>
-           let tmp := fresh_var "tmp" fvs in
            match nnrc_expr_to_nnrc_imp_expr e,
-                 nnrc_stmt_to_nnrc_imp_stmt_aux (tmp::x1::fvs) (Term_assign tmp) s1,
-                 nnrc_stmt_to_nnrc_imp_stmt_aux (tmp::x2::fvs) (Term_assign tmp) s2
+                 nnrc_stmt_to_nnrc_imp_stmt_aux fvs terminator s1,
+                 nnrc_stmt_to_nnrc_imp_stmt_aux fvs terminator s2
            with
            | Some e', Some s1', Some s2' =>
-             Some (NNRCimpLetMut
-                     tmp 
-                        (NNRCimpEither e' x1 s1' x2 s2')
-                        (terminate terminator (NNRCimpVar tmp)))
+             Some (NNRCimpEither e' x1 s1' x2 s2')
            | _, _, _ => None
            end
          | NNRCGroupBy _ _ _
@@ -190,8 +191,9 @@ Section NNRCtoNNRCimp.
     Definition nnrc_stmt_to_nnrc_imp_stmt (globals: list var) (stmt: nnrc) :
       option (nnrc_imp_stmt * var)
       :=
-        let ret := fresh_var "ret" globals in
-        match nnrc_stmt_to_nnrc_imp_stmt_aux (ret::globals) (Term_assign ret) stmt with
+        let fvs := globals ++ nnrc_bound_vars stmt in
+        let ret := fresh_var "ret" fvs in
+        match nnrc_stmt_to_nnrc_imp_stmt_aux (ret::fvs) (Term_assign ret) stmt with
         | Some stmt => Some (stmt, ret)
         | None => None
         end.
@@ -215,27 +217,23 @@ Section NNRCtoNNRCimp.
       - destruct (nnrc_expr_to_nnrc_imp_expr_stratified_some _ H) as [e eqe].
         rewrite eqe; simpl.
         eauto 2.
-      - destruct (IHs1 (v :: fvs) (Term_assign v) H)  as [s1' eqs1'].
-        destruct (IHs2 (v :: fvs) term H2)  as [s2' eqs2'].
+      - destruct (IHs1 fvs (Term_assign v) H)  as [s1' eqs1'].
+        destruct (IHs2 fvs term H2)  as [s2' eqs2'].
         rewrite eqs1', eqs2'; simpl.
         eauto 2.
       - destruct (nnrc_expr_to_nnrc_imp_expr_stratified_some _ H) as [e1 eqe1].
-        destruct (IHs2 (fresh_var "tmp" fvs :: v :: fvs)
+        destruct (IHs2 (fresh_var "tmp" fvs :: fvs)
                        (Term_push (fresh_var "tmp" fvs)) H2)  as [s1' eqs1'].
         rewrite eqe1, eqs1'; simpl.
         eauto 2.
       - destruct (nnrc_expr_to_nnrc_imp_expr_stratified_some _ H) as [e1 eqe1].
-        destruct (IHs2 (fresh_var "tmp" fvs :: fvs)
-                       (Term_assign (fresh_var "tmp" fvs)) H1)  as [s2' eqs2'].
-        destruct (IHs3 (fresh_var "tmp" fvs :: fvs)
-                       (Term_assign (fresh_var "tmp" fvs)) H3)  as [s3' eqs3'].
+        destruct (IHs2 fvs term H1)  as [s2' eqs2'].
+        destruct (IHs3 fvs term H3)  as [s3' eqs3'].
         rewrite eqe1, eqs2', eqs3'; simpl.
         eauto 2.
       - destruct (nnrc_expr_to_nnrc_imp_expr_stratified_some _ H) as [e1 eqe1].
-        destruct (IHs2 (fresh_var "tmp" fvs :: v :: fvs)
-                       (Term_assign (fresh_var "tmp" fvs)) H1)  as [s2' eqs2'].
-        destruct (IHs3 (fresh_var "tmp" fvs :: v0 :: fvs)
-                       (Term_assign (fresh_var "tmp" fvs)) H3)  as [s3' eqs3'].
+        destruct (IHs2 fvs term H1)  as [s2' eqs2'].
+        destruct (IHs3 fvs term H3)  as [s3' eqs3'].
         rewrite eqe1, eqs2', eqs3'; simpl.
         eauto 2.
       - destruct (nnrc_expr_to_nnrc_imp_expr_stratified_some _ H1) as [e1 eqe1].
@@ -252,10 +250,10 @@ Section NNRCtoNNRCimp.
       - unfold nnrc_stmt_to_nnrc_imp_stmt.
         intros cpf strats.
         destruct (nnrc_stmt_to_nnrc_imp_stmt_aux_stratified_some
-                    ((fresh_var "ret" fvs)::fvs)
-                    (Term_assign (fresh_var "ret" fvs)) _ strats) as [s' eqs'].
-      rewrite eqs' in cpf.
-      eauto 2.
+                    ((fresh_var "ret" (fvs ++ nnrc_bound_vars s))::fvs ++ nnrc_bound_vars s)
+                    (Term_assign (fresh_var "ret" (fvs ++ nnrc_bound_vars s))) _ strats) as [s' eqs'].
+        rewrite eqs' in cpf.
+        eauto 2.
     Defined.
     
     Definition stratified_nnrc_stmt_to_nnrc_imp_stmt fvs (s:nnrc)
@@ -268,6 +266,815 @@ Section NNRCtoNNRCimp.
          let nnrc_stratified_pf := NNRCStratify.stratify_stratified q in
          stratified_nnrc_stmt_to_nnrc_imp_stmt globals nnrc_stratified nnrc_stratified_pf.
 
+    (* Given a terminator and the returned states, 
+       determine what value was computed by the statement 
+     *)
+    
+    Definition get_terminator_result
+               (term:terminator)
+               (mc:mc_bindings)
+               (md:pd_bindings) : option data :=
+      match term with
+      | Term_assign v => olift id (lookup equiv_dec md v)
+      | Term_push v =>
+        match lookup equiv_dec mc v with
+        | Some xl => match rev xl with
+                     | x::xs => Some x
+                     | _ => None
+                     end
+        | _ => None
+        end
+      end.
+
+    Definition safe_terminator_result
+               (term:terminator)
+               (mc:mc_bindings)
+               (md:pd_bindings) : Prop :=
+      match term with
+      | Term_assign v => In v (domain md)
+      | Term_push v => In v (domain mc)
+      end.
+    
+    Lemma nnrc_imp_stmt_eval_terminator h σc pd mc md term e :
+      safe_terminator_result term mc md ->
+      match nnrc_imp_stmt_eval h σc pd mc md (terminate term e) with
+      | Some (pd', mc', md') =>
+        match get_terminator_result term mc' md' with
+        | Some res => nnrc_imp_expr_eval h σc pd e = Some res
+        | None => False
+        end
+      | None => nnrc_imp_expr_eval h σc pd e = None
+      end.
+    Proof.
+      destruct term; simpl; intros inn;
+        destruct (in_dom_lookup string_dec inn) as [dd eqdd];
+        rewrite eqdd
+        ; destruct (nnrc_imp_expr_eval h σc pd e); simpl; trivial
+        ; replace string_dec with
+              (@equiv_dec string (@eq string) (@eq_equivalence string) string_eqdec) by trivial
+        ;  rewrite lookup_update_eq_in by trivial
+        ; simpl; trivial.
+      rewrite rev_app_distr; simpl; trivial.
+    Qed.
+
+    Lemma nnrc_expr_to_nnrc_imp_expr_free_vars e ei :
+      nnrc_expr_to_nnrc_imp_expr e = Some ei ->
+      nnrc_free_vars e = nnrc_imp_expr_free_vars ei.
+    Proof.
+      revert ei.
+      induction e; simpl; intros ei eqq; invcs eqq; simpl; trivial.
+      - apply some_lift2 in H0.
+        destruct H0 as [? [??[??]]]; subst; simpl.
+        erewrite IHe1 by eauto.
+        erewrite IHe2 by eauto.
+        trivial.
+      - apply some_lift in H0.
+        destruct H0 as [???]; subst; simpl.
+        eauto.
+      - apply some_lift in H0.
+        destruct H0 as [???]; subst; simpl.
+        eauto.
+    Qed.
+
+    Local Open Scope string.
+    Require Import List.
+
+    Ltac match_option
+      := let eqq := fresh "eqq" in
+         match goal with
+           [|- context [match ?x with | Some _ => _ | None => _ end]] =>
+           case_eq x end; [ intros ? eqq | intros eqq]; rewrite eqq;
+         trivial; try discriminate.
+
+    Ltac match_option_in H
+      := let eqq := fresh "eqq" in
+         match type of H with
+           context [match ?x with | Some _ => _ | None => _ end] =>
+           case_eq x end; [ intros ? eqq | intros eqq]; rewrite eqq in H;
+         trivial; try discriminate.
+
+    Ltac expr_push_finisher ev x
+      := match_destr_in ev
+         ; simpl in ev
+         ; destruct (string_dec x x); [| congruence]
+         ; invcs ev
+         ; eauto.
+    
+    Lemma nnrc_stmt_to_nnrc_imp_stmt_aux_push1_assign_eq_mc 
+          s {si:nnrc_imp_stmt} {h σc pd mc md pd' mc' md'}:
+      nnrc_imp_stmt_eval h σc pd mc md si = Some (pd', mc', md') ->
+      (forall x fvs, nnrc_stmt_to_nnrc_imp_stmt_aux fvs (Term_push x) s = Some si ->
+                     forall mc2 old, mc = (x,old)::mc2 ->
+                                     exists n, mc' = ((x,old++n::nil)::mc2))
+      /\ 
+      (forall x fvs, nnrc_stmt_to_nnrc_imp_stmt_aux fvs (Term_assign x) s = Some si ->
+                     mc' = mc).
+    Proof.
+      revert si pd mc md pd' mc' md'.
+      nnrc_cases (induction s) Case;
+        intros si pd mc md pd' mc' md' ev;
+        (split; intros x fvs eqsi
+         ; [ intros mc2 old ?; subst; rename mc2 into mc | ])
+        ; simpl in eqsi; invcs eqsi
+        ; try solve [unfold nnrc_imp_stmt_eval in ev
+                     ; expr_push_finisher ev x
+                    | unfold nnrc_imp_stmt_eval in ev
+                      ; repeat match_destr_in ev
+                      ; invcs ev; trivial].
+      - Case "NNRCBinop".
+        match_option_in H0; try congruence.
+        apply some_lift2 in eqq.
+        destruct eqq as [?[? eqq1 [eqq2 H3]]].
+        invcs H0.
+        simpl in ev.
+        expr_push_finisher ev x.
+      - Case "NNRCBinop".
+        match_option_in H0.
+        invcs H0.
+        simpl in ev.
+        repeat match_option_in ev; try congruence.
+      - Case "NNRCUnop".
+        match_option_in H0.
+        apply some_lift in eqq.
+        destruct eqq as [? eq1 ?].
+        invcs H0.
+        simpl in ev.
+        expr_push_finisher ev x.
+      - Case "NNRCUnop".
+        match_option_in H0.
+        invcs H0.
+        simpl in ev.
+        repeat match_option_in ev; try congruence.
+      - Case "NNRCLet".
+        repeat match_option_in H0.
+        invcs H0.
+        simpl in ev.
+        repeat match_option_in ev.
+        destruct p as [[??]?].
+        destruct m0; try discriminate.
+        destruct p0.
+        repeat match_option_in ev.
+        destruct p0 as [[??]?].
+        destruct p0; try discriminate.
+        invcs ev.
+        destruct (IHs1 _ _ _ _ _ _ _ eqq1) as [IHs1p IHs1e].
+        destruct (IHs2 _ _ _ _ _ _ _ eqq2) as [IHs2p IHs2e].
+        eauto.
+      - Case "NNRCLet".
+        repeat match_option_in H0.
+        invcs H0.
+        simpl in ev.
+        repeat match_option_in ev.
+        destruct p as [[??]?].
+        destruct m0; try discriminate.
+        destruct p0.
+        repeat match_option_in ev.
+        destruct p0 as [[??]?].
+        destruct p0; try discriminate.
+        invcs ev.
+        destruct (IHs1 _ _ _ _ _ _ _ eqq1) as [IHs1p IHs1e].
+        destruct (IHs2 _ _ _ _ _ _ _ eqq2) as [IHs2p IHs2e].
+        specialize (IHs1e _ _ eqq).
+        specialize (IHs2e _ _ eqq0).
+        congruence.
+      - Case "NNRCFor".
+        repeat match_option_in H0.
+        invcs H0.
+        simpl in ev.
+        repeat match_option_in ev.
+        destruct p as [[??]?].
+        destruct m; try discriminate.
+        destruct p0.
+        repeat match_option_in ev.
+        destruct p0 as [[??]?].
+        destruct p0; try discriminate.
+        invcs ev.
+        destruct (equiv_dec (fresh_var "tmp" fvs) (fresh_var "tmp" fvs)); try congruence.
+        clear e.
+        unfold id in eqq2; simpl in eqq2.
+        match_option_in eqq2.
+        invcs eqq2.
+        match_option_in eqq1.
+        destruct d; try discriminate.
+        clear IHs1.
+        specialize (IHs2 n0).
+
+        cut ((forall l old s pd mc md pd' m md',
+                 (fix
+                  for_fun (dl : list data) (σ₁ : list (var * option data)) 
+                  (ψc₁ : mc_bindings) (ψd₁ : md_bindings) {struct dl} :
+                  option (list (var * option data) * mc_bindings * md_bindings) :=
+                  match dl with
+                  | nil => Some (σ₁, ψc₁, ψd₁)
+                  | d :: dl' =>
+                    match nnrc_imp_stmt_eval h σc ((v, Some d) :: σ₁) ψc₁ ψd₁ n0 with
+                    | Some (nil, _, _) => None
+                    | Some (_ :: σ₂, ψc₂, ψd₂) => for_fun dl' σ₂ ψc₂ ψd₂
+                    | None => None
+                    end
+                  end) l1 pd ((fresh_var "tmp" fvs, old) :: mc) md =
+               Some (pd', (s, l) :: m, md') ->
+                 exists n : list data, (s,l)::m = (fresh_var "tmp" fvs, old ++ n) :: mc)).
+        + intros HH.
+          apply (HH l nil) in eqq1.
+          destruct eqq1 as [? eqq5].
+          invcs eqq5.
+          simpl.
+          simpl in eqq3.
+          destruct (string_dec x x); [ | congruence].
+          invcs eqq3.
+          eauto.
+        + {
+            clear l pd pd' md md' old mc s n m l0 eqq1 eqq eqq2 eqq3.
+            induction l1; simpl; intros l old s pd mc md pd' m md' eqsi.
+            - invcs eqsi.
+              exists nil.
+              rewrite app_nil_r.
+              trivial.
+            - match_option_in eqsi.
+              destruct p as [[??]?].
+              destruct p; try discriminate.
+              specialize (IHs2 _ _ _ _ _ _ eqq).
+              destruct IHs2 as [IHs2p IHs2e].
+              specialize (IHs2p _ _ eqq0).
+              specialize (IHs2p _ _ (eq_refl)).
+              destruct IHs2p as [??]; subst.
+              specialize (IHl1 _ _ _ _ _ _ _ _ _ eqsi).
+              destruct IHl1 as [? eqq1].
+              invcs eqq1.
+              exists (x0::x1).
+              rewrite app_ass; simpl; trivial.
+            }
+      - Case "NNRCFor".
+        repeat match_option_in H0.
+        invcs H0.
+        simpl in ev.
+        repeat match_option_in ev.
+        destruct p as [[??]?].
+        destruct m; try discriminate.
+        destruct p0.
+        repeat match_option_in ev.
+        destruct p0 as [[??]?].
+        destruct p0; try discriminate.
+        invcs ev.
+        destruct (equiv_dec (fresh_var "tmp" fvs) (fresh_var "tmp" fvs)); try congruence.
+        clear e.
+        unfold id in eqq2; simpl in eqq2.
+        match_option_in eqq2.
+        invcs eqq2.
+        match_option_in eqq1.
+        destruct d; try discriminate.
+        clear IHs1.
+        specialize (IHs2 n0).
+
+        cut ((forall l old s pd mc md pd' m md',
+                 (fix
+                  for_fun (dl : list data) (σ₁ : list (var * option data)) 
+                  (ψc₁ : mc_bindings) (ψd₁ : md_bindings) {struct dl} :
+                  option (list (var * option data) * mc_bindings * md_bindings) :=
+                  match dl with
+                  | nil => Some (σ₁, ψc₁, ψd₁)
+                  | d :: dl' =>
+                    match nnrc_imp_stmt_eval h σc ((v, Some d) :: σ₁) ψc₁ ψd₁ n0 with
+                    | Some (nil, _, _) => None
+                    | Some (_ :: σ₂, ψc₂, ψd₂) => for_fun dl' σ₂ ψc₂ ψd₂
+                    | None => None
+                    end
+                  end) l0 pd ((fresh_var "tmp" fvs, old) :: mc) md =
+                 Some (pd', (s, l) :: m, md') ->
+                 exists n : list data, (s,l)::m = (fresh_var "tmp" fvs, old ++ n) :: mc)).
+        + intros HH.
+          apply (HH l nil) in eqq1.
+          destruct eqq1 as [? eqq5].
+          invcs eqq5.
+          simpl.
+          simpl in eqq3.
+          destruct (string_dec x x); [ | congruence].
+          invcs eqq3.
+          eauto.
+        +
+            clear l pd pd' md m0 mc s n eqq1 eqq eqq2 eqq3. 
+          {
+            induction l0; simpl; intros l old s pd mc md pd' m md' eqsi.
+            - invcs eqsi.
+              exists nil.
+              rewrite app_nil_r.
+              trivial.
+            - match_option_in eqsi.
+              destruct p as [[??]?].
+              destruct p; try discriminate.
+              specialize (IHs2 _ _ _ _ _ _ eqq).
+              destruct IHs2 as [IHs2p IHs2e].
+              specialize (IHs2p _ _ eqq0).
+              specialize (IHs2p _ _ (eq_refl)).
+              destruct IHs2p as [??]; subst.
+              specialize (IHl0 _ _ _ _ _ _ _ _ _ eqsi).
+              destruct IHl0 as [? eqq1].
+              invcs eqq1.
+              exists (x0::x1).
+              rewrite app_ass; simpl; trivial.
+            }
+      - Case "NNRCIf".
+        repeat match_option_in H0.
+        invcs H0.
+        simpl in ev.
+        repeat match_option_in ev.
+        destruct d; try discriminate.
+        destruct b.
+        + destruct (IHs2 _ _ _ _ _ _ _ ev) as [IHs2p IHs2e]; eauto.
+        + destruct (IHs3 _ _ _ _ _ _ _ ev) as [IHs3p IHs3e]; eauto.
+      - Case "NNRCIf".
+        repeat match_option_in H0.
+        invcs H0.
+        simpl in ev.
+        repeat match_option_in ev.
+        destruct d; try discriminate.
+        destruct b.
+        + destruct (IHs2 _ _ _ _ _ _ _ ev) as [IHs2p IHs2e]; eauto.
+        + destruct (IHs3 _ _ _ _ _ _ _ ev) as [IHs3p IHs3e]; eauto.
+      - Case "NNRCEither".
+        repeat match_option_in H0.
+        invcs H0.
+        simpl in ev.
+        repeat match_option_in ev.
+        destruct d; try discriminate
+        ; repeat match_option_in ev
+        ; destruct p as [[??]?]; destruct p; try discriminate
+        ; invcs ev.
+        + destruct (IHs2 _ _ _ _ _ _ _ eqq3) as [IHs2p IHs2e]; eauto.
+        + destruct (IHs3 _ _ _ _ _ _ _ eqq3) as [IHs3p IHs3e]; eauto.
+      - Case "NNRCEither".
+        repeat match_option_in H0.
+        invcs H0.
+        simpl in ev.
+        repeat match_option_in ev.
+        destruct d; try discriminate
+        ; repeat match_option_in ev
+        ; destruct p as [[??]?]; destruct p; try discriminate
+        ; invcs ev.
+        + destruct (IHs2 _ _ _ _ _ _ _ eqq3) as [IHs2p IHs2e]; eauto.
+        + destruct (IHs3 _ _ _ _ _ _ _ eqq3) as [IHs3p IHs3e]; eauto.
+      - Case "NNRCGroupBy".
+        match_option_in H0.
+        invcs H0.
+        unfold nnrc_imp_stmt_eval in ev.
+        expr_push_finisher ev x.
+      - Case "NNRCGroupBy".
+        match_option_in H0.
+        invcs H0.
+        unfold nnrc_imp_stmt_eval in ev.
+        repeat match_destr_in ev.
+        invcs ev; trivial.
+    Qed.
+
+    Lemma nnrc_stmt_to_nnrc_imp_stmt_aux_assign_eq 
+          {s:nnrc} {fvs} {si:nnrc_imp_stmt} {h σc pd mc md x pd' mc' md'}:
+      nnrc_imp_stmt_eval h σc pd mc md si = Some (pd', mc', md') ->
+      nnrc_stmt_to_nnrc_imp_stmt_aux fvs (Term_assign x) s = Some si ->
+      mc' = mc.
+    Proof.
+      intros eqsi ev.
+      destruct (nnrc_stmt_to_nnrc_imp_stmt_aux_push1_assign_eq_mc s eqsi).
+      eauto.
+    Qed.
+    
+    Lemma nnrc_stmt_to_nnrc_imp_stmt_aux_push1 
+          {s:nnrc} {fvs} {si:nnrc_imp_stmt} {h σc pd mc md x pd' mc' md' old}:
+      nnrc_imp_stmt_eval h σc pd ((x,old)::mc) md si = Some (pd', mc', md') ->
+      nnrc_stmt_to_nnrc_imp_stmt_aux fvs (Term_push x) s = Some si ->
+      exists n, mc' = ((x,old++n::nil)::mc).
+    Proof.
+      intros eqsi ev.
+      destruct (nnrc_stmt_to_nnrc_imp_stmt_aux_push1_assign_eq_mc s eqsi).
+      eauto.
+    Qed.
+
+    Lemma nnrc_stmt_to_nnrc_imp_stmt_aux_some_correct
+          {s:nnrc} {fvs term} {si:nnrc_imp_stmt} :
+      nnrc_stmt_to_nnrc_imp_stmt_aux fvs term s = Some si ->
+      forall h σc σ mc md,
+        incl (domain σ) fvs ->
+        incl (domain mc) fvs ->
+        incl (nnrc_bound_vars s) fvs ->
+        safe_terminator_result term mc md ->
+        let ne := @nnrc_eval _ h σc σ s in
+        match nnrc_imp_stmt_eval h σc (pd_bindings_lift σ) mc md si with
+        | None => ne = None
+        | Some (pd', mc', md') =>
+          match get_terminator_result term mc' md' with
+          | Some res => ne = Some res
+          | None => False
+          end
+        end.
+    Proof.
+      unfold nnrc_eval.
+      intros eqsi h σc.
+      revert fvs term si eqsi; simpl.
+      nnrc_cases (induction s) Case; intros fvs term si eqsi σ mc md inclσ inclmc inclbvars safe_term.
+      - Case "NNRCGetConstant".
+        invcs eqsi; simpl; intros.
+        apply nnrc_imp_stmt_eval_terminator; trivial.
+      - Case "NNRCVar".
+        invcs eqsi.
+        generalize (nnrc_imp_stmt_eval_terminator h σc (pd_bindings_lift σ) mc md term (NNRCimpVar v) safe_term); intros eterm.
+        match_destr; simpl in *.
+        + destruct p as [[??]?].
+          match_destr.
+          rewrite lookup_pd_bindings_lift, olift_id_lift_some in eterm; trivial.
+        + rewrite lookup_pd_bindings_lift, olift_id_lift_some in eterm; trivial.
+      - Case "NNRCConst".
+        invcs eqsi.
+        apply nnrc_imp_stmt_eval_terminator; trivial.
+      - Case "NNRCBinop".
+        simpl in *.
+        case_eq (nnrc_expr_to_nnrc_imp_expr s1); [intros s1' s1'eq | intros s1'eq]
+        ; rewrite s1'eq in eqsi; try discriminate.
+        case_eq (nnrc_expr_to_nnrc_imp_expr s2); [intros s2' s2'eq | intros s2'eq]
+        ; rewrite s2'eq in eqsi; try discriminate.
+        simpl in eqsi; invcs eqsi.
+        generalize (nnrc_imp_stmt_eval_terminator h σc (pd_bindings_lift σ) mc md term (NNRCimpBinop b s1' s2') safe_term); intros eterm.
+        rewrite (nnrc_expr_to_nnrc_imp_expr_some_correct' _ _ s1'eq).
+        rewrite (nnrc_expr_to_nnrc_imp_expr_some_correct' _ _ s2'eq).
+        eauto.
+      - Case "NNRCUnop".
+        simpl in *.
+        case_eq (nnrc_expr_to_nnrc_imp_expr s); [intros s1' s1'eq | intros s1'eq]
+        ; rewrite s1'eq in eqsi; try discriminate.
+        simpl in eqsi; invcs eqsi.
+        generalize (nnrc_imp_stmt_eval_terminator h σc (pd_bindings_lift σ) mc md term (NNRCimpUnop u s1' ) safe_term); intros eterm.
+        rewrite (nnrc_expr_to_nnrc_imp_expr_some_correct' _ _ s1'eq).
+        eauto.
+      - Case "NNRCLet".
+        simpl in *.
+        match_case_in eqsi; [ intros ? eqq1 | intros eqq1]
+        ; rewrite eqq1 in eqsi; try discriminate.
+        match_case_in eqsi; [ intros ? eqq2 | intros eqq2]
+        ; rewrite eqq2 in eqsi; try discriminate.
+        invcs eqsi; simpl.
+        specialize (IHs1 _ _ _ eqq1).
+        specialize (IHs1 σ mc ((v, None) :: md)).
+        cut_to IHs1; simpl; eauto 4.
+        + match_case_in IHs1; [intros ? eqq3 | intros eqq3]
+          ; rewrite eqq3 in IHs1; [ | rewrite IHs1; trivial].
+          destruct p as [[??]?].
+          simpl in IHs1.
+          match_case_in IHs1; [intros ? eqq4 | intros eqq4]
+          ; rewrite eqq4 in IHs1; [| tauto].
+          unfold id in eqq4; apply some_olift in eqq4; simpl in eqq4.
+          destruct eqq4 as [? eqq4 ?]; subst.
+          rewrite IHs1.
+          generalize (nnrc_imp_stmt_eval_env_stack eqq3); intros; subst.
+          generalize (nnrc_imp_stmt_eval_mcenv_domain_stack eqq3); intros eqq5.
+          generalize (nnrc_imp_stmt_eval_mdenv_domain_stack eqq3); intros eqq6.
+          destruct m0; simpl in *; try discriminate.
+          destruct p; simpl in *.
+          invcs eqq6.
+          match_destr_in eqq4; [clear e | congruence].
+          invcs eqq4.
+          specialize (IHs2 _ _ _ eqq2).
+          specialize (IHs2 ((s, d) :: σ) m m0).
+          cut_to IHs2.
+          * {
+              match_case_in IHs2; [intros ? eqq7 | intros eqq7]
+              ; rewrite eqq7 in IHs2; simpl in eqq7
+              ; unfold var in *; rewrite eqq7; trivial.
+              destruct p as [[??]?].
+              match_case_in IHs2;
+                [intros ? eqq8 | intros eqq8]
+                ; rewrite eqq8 in IHs2; try tauto.
+              rewrite IHs2.
+              generalize (nnrc_imp_stmt_eval_env_stack eqq7); intros; subst.
+              rewrite eqq8; trivial.
+            }
+          * simpl; intuition.
+          * unfold var in *.
+            rewrite <- eqq5; trivial.
+          * unfold incl in *; simpl in inclbvars.
+            intros ??; apply inclbvars.
+            rewrite in_app_iff; intuition.
+          * unfold safe_terminator_result in *.
+            rewrite <- eqq5.
+            rewrite <- H1.
+            trivial.
+        + unfold incl in *; simpl in inclbvars.
+          intros ??; apply inclbvars.
+          rewrite in_app_iff; intuition.
+      - Case "NNRCFor".
+        simpl in *.
+        case_eq (nnrc_expr_to_nnrc_imp_expr s1); [intros s1' s1'eq | intros s1'eq]
+        ; rewrite s1'eq in eqsi; try discriminate.
+        rewrite (nnrc_expr_to_nnrc_imp_expr_some_correct' _ _ s1'eq).
+        match_case_in eqsi; [ intros ? eqq1 | intros eqq1]
+        ; rewrite eqq1 in eqsi; try discriminate.
+        invcs eqsi.
+        simpl.
+        destruct (nnrc_imp_expr_eval h σc (pd_bindings_lift σ) s1'); trivial.
+        destruct d; trivial.
+        clear s1' IHs1 s1'eq.
+        specialize (IHs2 _ _ _ eqq1).
+
+        cut (forall old, match
+                  match
+                    (fix
+                       for_fun (dl : list data) (σ₁ : list (var * option data)) 
+                       (ψc₁ : mc_bindings) (ψd₁ : md_bindings) {struct dl} :
+                       option (list (var * option data) * mc_bindings * md_bindings) :=
+                       match dl with
+                       | nil => Some (σ₁, ψc₁, ψd₁)
+                       | d :: dl' =>
+                         match nnrc_imp_stmt_eval h σc ((v, Some d) :: σ₁) ψc₁ ψd₁ n with
+                         | Some (nil, _, _) => None
+                         | Some (_ :: σ₂, ψc₂, ψd₂) => for_fun dl' σ₂ ψc₂ ψd₂
+                         | None => None
+                         end
+                       end) l (pd_bindings_lift σ) ((fresh_var "tmp" fvs, old) :: mc) md
+                  with
+                  | Some (σ₁, nil, _) => None
+                  | Some (σ₁, (_, dl) :: ψc₁, ψd₁) =>
+                    match
+                      nnrc_imp_stmt_eval h σc ((fresh_var "tmp" fvs, Some (dcoll dl)) :: σ₁) ψc₁ ψd₁
+                                         (terminate term (NNRCimpVar (fresh_var "tmp" fvs)))
+                    with
+                    | Some (nil, _, _) => None
+                    | Some (_ :: σ₂, ψc₂, ψd₂) => Some (σ₂, ψc₂, ψd₂)
+                    | None => None
+                    end
+                  | None => None
+                  end
+                with
+                | Some (_, mc', md') =>
+                  match get_terminator_result term mc' md' with
+                  | Some res =>
+                    lift (fun x => dcoll (old ++ x))
+                         (lift_map
+                            (fun d1 : data => nnrc_core_eval h σc ((v, d1) :: σ) (nnrc_to_nnrc_base s2))
+                            l) = Some res
+                  | None => False
+                  end
+                | None =>
+                  lift dcoll
+                       (lift_map
+                          (fun d1 : data => nnrc_core_eval h σc ((v, d1) :: σ) (nnrc_to_nnrc_base s2)) l) =
+                  None
+                end).
+        { unfold var in *.
+          intros HH; specialize (HH nil); simpl in HH.
+          trivial.
+        } 
+        revert σ mc md inclσ inclmc safe_term.
+        induction l; simpl; intros.
+        + generalize (nnrc_imp_stmt_eval_terminator h σc ((fresh_var "tmp" fvs, Some (dcoll old)) :: pd_bindings_lift σ) mc md term (NNRCimpVar (fresh_var "tmp" fvs)) safe_term); intros eterm.
+          unfold var in *.
+          match_case_in eterm; [intros ? eqq2 | intros eqq2]
+          ; rewrite eqq2 in eterm; try tauto.
+          * destruct p as [[??]?].
+            match_case_in eterm; [intros ? eqq3 | intros eqq3]
+            ; rewrite eqq3 in eterm; try tauto.
+            generalize (nnrc_imp_stmt_eval_env_stack eqq2); intros; subst.
+            rewrite eqq3.
+            simpl in eterm.
+            rewrite app_nil_r.
+            match_destr_in eterm.
+            unfold id in eterm.
+            congruence.
+          * simpl in eterm.
+            unfold id in eterm.
+            match_destr_in eterm.
+            congruence.
+        + specialize (IHs2 ((v, a) :: σ) ((fresh_var "tmp" fvs, old) :: mc) md).
+          cut_to IHs2.
+          * simpl in IHs2.
+            match_case_in IHs2; [intros ? eqq7 | intros eqq7]
+            ; rewrite eqq7 in IHs2; simpl in eqq7
+            ; unfold var in *; rewrite eqq7
+            ; [ | rewrite IHs2; simpl; trivial].
+            destruct p as [[??]?].
+            match_case_in IHs2;
+              [intros ? eqq8 | intros eqq8]
+              ; rewrite eqq8 in IHs2; try tauto.
+            rewrite IHs2.
+            generalize (nnrc_imp_stmt_eval_env_stack eqq7); intros; subst.            
+            generalize (nnrc_imp_stmt_eval_mcenv_domain_stack eqq7); intros mceqq.
+            destruct m; simpl in mceqq; try discriminate.
+            destruct p; simpl in *.
+            invcs mceqq.
+            destruct (equiv_dec (fresh_var "tmp" fvs) (fresh_var "tmp" fvs)); [| congruence].
+            destruct l0; try discriminate.
+            invcs eqq8.
+            match_case_in H0
+            ; [intros eqq0 | intros ? ? eqq0]
+            ; rewrite eqq0 in H0; try discriminate.
+            invcs H0.
+            assert (eqq0':d0::l0 = rev (d :: l1)).
+            { rewrite <- eqq0.
+              rewrite rev_app_distr.
+              rewrite rev_involutive; simpl; trivial.
+            }
+            rewrite eqq0'.
+            generalize (nnrc_stmt_to_nnrc_imp_stmt_aux_push1 eqq7 eqq1); intros [? eqqq].
+            invcs eqqq.
+            rewrite eqq0' in H0.
+            assert (eqqq':d::l1 = rev (old ++ x :: nil)).
+            { rewrite <- H0; rewrite rev_involutive; trivial. }
+            rewrite rev_app_distr in eqqq'; simpl in eqqq'.
+            clear H0.
+            invcs eqqq'.
+            specialize (IHl σ mc m0).
+            {
+              cut_to IHl; trivial.
+              - unfold var in *.
+                simpl.
+                rewrite rev_involutive.
+                specialize (IHl (old ++ x :: nil)).
+                match goal with
+                  [H:match (match ?x with | _ => _ end ) with | _ => _ end |- _] =>
+                  let eqq := (fresh "eqq") in
+                  case_eq x
+                  ;           [intros ? eqq | intros eqq]
+                  ; rewrite eqq in H; try tauto
+                end.
+                + destruct p as [[??]?].
+                  destruct m.
+                  * apply none_lift in IHl.
+                    rewrite IHl; simpl; trivial.
+                  * destruct p.
+                    { 
+                      match goal with
+                        [H:match (match ?x with | _ => _ end ) with | _ => _ end |- _] =>
+                        let eqq := (fresh "eqq") in
+                        case_eq x
+                        ;           [intros ? eqq | intros eqq]
+                        ; rewrite eqq in H; try tauto
+                      end.
+                      - destruct p as [[??]?].
+                        destruct p.
+                        + apply none_lift in IHl.
+                          rewrite IHl; simpl; trivial.
+                        + match_case_in IHl;
+                            [intros ? eqq3 | intros eqq3]
+                            ; rewrite eqq3 in IHl; try tauto.
+                          apply some_lift in IHl.
+                          destruct IHl as [? eqq4 ?]; subst.
+                          rewrite eqq4.
+                          simpl.
+                          rewrite <- app_assoc; simpl; trivial.
+                      - apply none_lift in IHl.
+                        rewrite IHl; simpl; trivial.
+                    } 
+                + apply none_lift in IHl.
+                  rewrite IHl; simpl; trivial.
+              - generalize (nnrc_imp_stmt_eval_mdenv_domain_stack eqq7); intros mdeqq.
+                unfold safe_terminator_result in *; rewrite <- mdeqq; trivial.
+            }
+          * unfold incl in *; simpl in *; intuition.
+          * unfold incl in *; simpl in *; intuition.
+          * unfold incl in *; simpl in inclbvars; intros.
+            right. apply inclbvars.
+            rewrite in_app_iff; intuition.
+          * simpl; intuition.
+      - Case "NNRCIf".
+        simpl in *.
+        case_eq (nnrc_expr_to_nnrc_imp_expr s1); [intros s1' s1'eq | intros s1'eq]
+        ; rewrite s1'eq in eqsi; try discriminate.
+        rewrite (nnrc_expr_to_nnrc_imp_expr_some_correct' _ _ s1'eq).
+        match_case_in eqsi; [ intros ? eqq1 | intros eqq1]
+        ; rewrite eqq1 in eqsi; try discriminate.
+        match_case_in eqsi; [ intros ? eqq2 | intros eqq2]
+        ; rewrite eqq2 in eqsi; try discriminate.
+        invcs eqsi.
+        simpl.
+        destruct (nnrc_imp_expr_eval h σc (pd_bindings_lift σ) s1' )
+        ; simpl; trivial.
+        destruct d; simpl; trivial.
+        destruct b.
+        + eapply IHs2; eauto.
+          unfold incl in *; simpl in inclbvars.
+          intros ??; apply inclbvars.
+          rewrite in_app_iff; intuition.
+        + eapply IHs3; eauto. 
+          unfold incl in *; simpl in inclbvars.
+          intros ??; apply inclbvars.
+          rewrite in_app_iff; intuition.
+      - Case "NNRCEither".
+        simpl in *.
+        case_eq (nnrc_expr_to_nnrc_imp_expr s1); [intros s1' s1'eq | intros s1'eq]
+        ; rewrite s1'eq in eqsi; try discriminate.
+        rewrite (nnrc_expr_to_nnrc_imp_expr_some_correct' _ _ s1'eq).
+        match_case_in eqsi; [ intros ? eqq1 | intros eqq1]
+        ; rewrite eqq1 in eqsi; try discriminate.
+        match_case_in eqsi; [ intros ? eqq2 | intros eqq2]
+        ; rewrite eqq2 in eqsi; try discriminate.
+        invcs eqsi.
+        simpl.
+        destruct (nnrc_imp_expr_eval h σc (pd_bindings_lift σ) s1' )
+        ; simpl; trivial.
+        destruct d; simpl; trivial.
+        + specialize (IHs2 _ _ _ eqq1).
+          specialize (IHs2 ((v, d) :: σ) mc md).
+          cut_to IHs2; intuition.
+          * match_case_in IHs2; [intros ? eqq3 | intros eqq3]
+            ; rewrite eqq3 in IHs2
+            ; simpl in eqq3; unfold var in *; rewrite eqq3; trivial.
+            destruct p as [[??]?].
+            generalize (nnrc_imp_stmt_eval_env_stack eqq3); intros; subst.
+            eauto.
+          * simpl; unfold incl in *.
+            simpl in *; intuition.
+          * simpl; unfold incl in *.
+            intros; apply inclbvars.
+            simpl; repeat rewrite in_app_iff; intuition.
+        + specialize (IHs3 _ _ _ eqq2).
+          specialize (IHs3 ((v0, d) :: σ) mc md).
+          cut_to IHs3; intuition.
+          * match_case_in IHs3; [intros ? eqq3 | intros eqq3]
+            ; rewrite eqq3 in IHs3
+            ; simpl in eqq3; unfold var in *; rewrite eqq3; trivial.
+            destruct p as [[??]?].
+            generalize (nnrc_imp_stmt_eval_env_stack eqq3); intros; subst.
+            eauto.
+          * simpl; unfold incl in *.
+            simpl in *; intuition.
+          * simpl; unfold incl in *.
+            intros; apply inclbvars.
+            simpl; repeat rewrite in_app_iff; intuition.
+      - Case "NNRCGroupBy".
+        simpl in eqsi.
+        case_eq (nnrc_expr_to_nnrc_imp_expr s0); [intros s1' s1'eq | intros s1'eq]
+        ; rewrite s1'eq in eqsi; simpl in eqsi; try discriminate.
+        invcs eqsi.
+        generalize (nnrc_imp_stmt_eval_terminator h σc (pd_bindings_lift σ) mc md term (NNRCimpGroupBy s l s1') safe_term); intros eterm.
+        simpl nnrc_to_nnrc_base.
+        match_destr_in eterm.
+        + destruct p as [[??]?].
+          match_destr.
+          simpl nnrc_to_nnrc_base.
+          simpl in eterm.
+          rewrite <- (nnrc_expr_to_nnrc_imp_expr_some_correct' _ _ s1'eq) in eterm.
+          match_case_in eterm; [intros ? eqq1 | intros eqq1]
+          ; rewrite eqq1 in eterm
+          ; simpl in eqq1; try discriminate.
+          destruct d0; try discriminate.
+          erewrite nnrc_group_by_correct; eauto.
+        + simpl in eterm.
+          match_case_in eterm; [intros ? eqq1 | intros eqq1]
+          ; rewrite eqq1 in eterm
+          ; simpl in eqq1.
+          * rewrite <- (nnrc_expr_to_nnrc_imp_expr_some_correct' _ _ s1'eq) in eqq1.
+            destruct d;
+              (try solve[
+                     eapply nnrc_group_by_correct_some_ncoll; eauto; intros; discriminate]).
+            erewrite nnrc_group_by_correct; eauto.
+          * rewrite <- (nnrc_expr_to_nnrc_imp_expr_some_correct' _ _ s1'eq) in eqq1.
+            eapply nnrc_group_by_correct_none; eauto.
+    Qed.
+    
+    Lemma nnrc_to_nnrc_imp_some_correct
+          h σc {s:nnrc} {globals} {si:nnrc_imp} {ret:var} :
+      nnrc_stmt_to_nnrc_imp_stmt globals s = Some si ->
+      @nnrc_eval _ h σc nil s = nnrc_imp_eval_top h σc si.
+    Proof.
+      unfold nnrc_stmt_to_nnrc_imp_stmt, nnrc_imp_eval_top.
+      intros eqsi.
+      destruct si.
+      match_option_in eqsi.
+      invcs eqsi.
+      generalize (nnrc_stmt_to_nnrc_imp_stmt_aux_some_correct
+                    eqq
+                    h σc nil nil
+                    ((fresh_var "ret" (globals ++ nnrc_bound_vars s), None) :: nil)
+                 ); intros HH.
+      simpl in HH.
+      unfold var in *.
+      cut_to HH; try solve [ unfold incl; simpl; tauto].
+      - match_option_in HH.
+        destruct p as [[??]?].
+        generalize (nnrc_imp_stmt_eval_mdenv_domain_stack eqq0); intros mceqq.
+        simpl in mceqq.
+        destruct m0; try discriminate.
+        simpl in mceqq; invcs mceqq.
+        destruct m0; try discriminate.
+        destruct p0; simpl in *; subst.
+        destruct ( equiv_dec (fresh_var "ret" (globals ++ nnrc_bound_vars s))
+                             (fresh_var "ret" (globals ++ nnrc_bound_vars s))); try congruence.
+        unfold id in HH; simpl in HH.
+        destruct o; try tauto.
+      - unfold incl; simpl; intros.
+        repeat rewrite in_app_iff; intuition.
+    Qed.
+    
+    Section tests.
+      Local Open Scope nnrc_scope.
+      Local Open Scope string_scope.
+
+      Example nnrc1 := (‵abs ‵ (dnat 3) ‵+ ‵(dnat 5)) ‵+ ((‵(dnat 4) ‵+ ‵(dnat 7)) ‵+‵`(dnat  3)).
+      (*    Eval vm_compute in (stratify nnrc1). *)
+
+      Example nnrc2 := NNRCLet "x" (NNRCLet "x" (‵ (dnat 3) ‵+ ‵(dnat 5)) (NNRCVar "x")) (NNRCVar "x").
+      (* Eval vm_compute in (nnrc_to_nnrc_imp_top nil nnrc2). *)
+    End tests.
+
   End from_stratified.
 
+
+  
 End NNRCtoNNRCimp.
